theories/LVal.v
@@ -1,0 +1,5 @@
+Require Import Variables.
+
+Inductive lval : Type :=
+| LVar : Var.t -> lval 
+| LDeref : lval -> lval.
