theories/Lattice.v
@@ -1,0 +1,45 @@
+(************************************************************************)
+(* Copyright 2022 Frédéric Dabrowski                                    *)
+(* 
+    This program is free software:: you can redistribute it and/or modify
+    it under the terms of the GNU General Public License as published by
+    the Free Software Foundation, either version 3 of the License, or
+    (at your option) any later version.
+
+    Foobar is distributed in the hope that it will be useful,
+    but WITHOUT ANY WARRANTY; without even the implied warranty of
+    MERCHANTABILITY or FITNESS FOR A PARTICULAR PURPOSE.  See the
+    GNU General Public License for more details.
+
+    You should have received a copy of the GNU General Public License
+    along with Foobar.  If not, see <https://www.gnu.org/licenses/>.    *)
+(************************************************************************)
+
+(** * Lattices *)
+
+Require Import Coq.Relations.Relation_Definitions.
+Require Import Coq.Classes.RelationClasses.
+
+Class JoinLattice {A : Type} (eqA : relation A) `{equ : Equivalence A eqA}
+(R : relation A) `{partialOrder : PartialOrder A eqA R} (join : A -> A -> A)  :=
+{
+    join_bound1 (x y : A) : R x (join x y);
+    join_bound2 (x y : A) : R y (join x y);
+    join_least_upper_bound (x y z : A) : R x z -> R y z -> R (join x y) z 
+}.
+
+Class MeetLattice {A : Type} (eqA : relation A) `{equ : Equivalence A eqA}
+(R : relation A) `{partialOrder : PartialOrder A eqA R} (meet : A -> A -> A)  :=
+{
+    meet_bound1 (x y : A) : R (meet x y) x;
+    meet_bound2 (x y : A) : R (meet x y) y;
+    meet_greatest_lower_bound (x y z : A) : R z x -> R z y -> R z (meet x y)
+}.
+
+Class Lattice {A : Type} (eqA : relation A) `{equ : Equivalence A eqA}
+(R : relation A) `{partialOrder : PartialOrder A eqA R}
+(join : A -> A -> A) (meet : A -> A -> A): Type :=
+{
+    Lattice_JoinLattice :> JoinLattice eqA R join; 
+    Lattice_MeetLattice :> MeetLattice  eqA R meet
+}.
