theories/LatticeExamples.v
@@ -1,0 +1,82 @@
+
+Definition eqb (b1 b2 : bool) : Prop := b1 = b2.
+Definition ltb (b1 b2 : bool) : Prop := 
+    match (b1, b2) with 
+        | (false, _) => True
+        | (true, true) => True
+        | (true, talse) => False 
+        end.
+
+#[export] Instance ref_eqb : Reflexive eqb.
+constructor.
+Qed.
+
+#[export] Instance sym_eqb : Symmetric eqb.
+intros x y  H.
+symmetry.
+assumption.
+Qed.
+
+#[export] Instance trans_eqb : Transitive eqb.
+intros x y z H1 H2.
+transitivity y.
+assumption.
+assumption.
+Qed.
+
+#[export] Instance eq_eqb : Equivalence eqb.
+constructor.
+apply ref_eqb.
+apply sym_eqb.
+apply trans_eqb.
+Qed.
+
+#[export] Instance refl_ltb : Reflexive ltb.
+intros x.
+unfold ltb.
+case_eq x; intros; subst.
+trivial.
+trivial.
+Qed.
+
+#[export] Instance trans_ltb : Transitive ltb.
+intros x y z H1 H2.
+destruct x,y,z;  trivial.
+Qed.
+
+#[export] Instance preo_eqb : PreOrder ltb.
+constructor.
+apply refl_ltb.
+apply trans_ltb.
+Qed.
+
+#[export] Instance po : PartialOrder eqb ltb.
+constructor.
+-   unfold eqb, ltb, Basics.flip.
+    split; destruct x, x0; solve [trivial | discriminate].
+-   unfold eqb, ltb, Basics.flip.
+    intros [H1 H2].
+    destruct x, x0; intuition.
+Qed.
+
+Definition joinb (b1 b2 : bool) : bool :=
+    match (b1, b2) with 
+        | (false, false) => false
+        | (_, _) => true 
+        end.
+
+#[global] Instance jl : JoinLattice eqb ltb joinb.
+constructor.
+-   intros; unfold ltb, joinb.
+    destruct x, y; trivial.
+-   intros; unfold ltb, joinb.
+    destruct x, y; trivial.
+- intros; unfold ltb, joinb.
+    destruct x, y, z; trivial.
+Defined.
+
+Lemma a : forall b1 b2 : bool, ltb b1 (joinb b1 b2).
+Proof.
+    intros.
+    apply join_bound1.
+Qed.
