theories/Lifetime.v
@@ -1,0 +1,18 @@
+Require Import Lattice.
+Require Import Coq.Relations.Relation_Definitions.
+Require Import Coq.Classes.RelationClasses.
+
+Module Lifetime.
+
+    Parameter t : Type.
+    Parameter glob : t.
+    Parameter eq : relation t.
+    Parameter lt : relation t.
+    Parameter join : t -> t -> t.
+
+    #[export] Declare Instance k : Equivalence eq.
+    #[export] Declare Instance j : PreOrder lt.
+    #[export] Declare Instance m : PartialOrder eq lt.
+    #[export] Declare Instance i : MeetLattice eq lt join.
+
+End Lifetime.
