theories/Semantics.v
@@ -1,6 +1,5 @@
 From MSSL Require Import Syntax.
 Require Import Coq.FSets.FMapList.
-Require Import Coq.Structures.OrderedType.
 Require Import Coq.Structures.OrdersEx.
 Require Import Coq.Arith.PeanoNat.
 Require Import Coq.Structures.OrderedTypeEx.
@@ -10,45 +9,50 @@ Require Import Relations.
 
 Require Import List.
 Import ListNotations.
-Require Import String.
+Require Import Variables.
 
-Require Import Monoid.
+Require Import Monoid MonoidExamples.
 Require Import Functor.
 Require Import Coq.Sets.Ensembles.
 Open Scope type_scope.
 
-Definition transition (A B : Type) := A -> B -> A -> Prop.
+Require Import Coq.Program.Basics.
 
-Inductive tr_clos_rt (A B : Type) {MB : Monoid B}(T : transition A B) : transition A B :=   
-| tr_close_rt_step : forall x y z,
-    T x y z -> tr_clos_rt A B T x y z
-| tr_close_rt_refl : forall a,
-        tr_clos_rt A B T a mempty a
-| tr_close_rt_trans : forall x a y b z,
-    T x a y -> T x b z -> tr_clos_rt A B T x (mappend a b) z.
+Require Import Lifetime Store LVal Value.
 
-Module Semantics (Lifetime : BoundedOrderedType).
+Require Import Transition.
 
-    Module Import S := MSSLSyntax(Lifetime).
-    Import S.V.
+Require Import Monad.
+Open Scope monad_scope.
 
+
+Open Scope type_scope.
    
+    Import MSSLSyntax.
+    Import Value.
+
+    Module D <: StoreDomain. 
+        Definition loc := location.
+        Definition val := partialValue * sum Lifetime.t nat.
+    End D.
+
+    Module S := Store (D).
 
     Definition isValue (e : expression) : Prop :=
             match e with EVal v => True | _ => False end.
 
-    Definition getValue (e : expression) (H : isValue e) : value :=
-        match e as e0 return (isValue e0 -> value) with 
+    Definition getValue (e : expression) (H : isValue e) : Value.value :=
+        match e as e0 return (isValue e0 -> Value.value) with 
             | EVal v => const v
-            | e' => False_rect _ 
+            | _ => False_rect _ 
         end H.
 
 
 
 
-    Coercion EVal : value >-> expression.
+    Coercion EVal : Value.value >-> expression.
 
-    Axiom instantiate : Store.t -> Lifetime.t -> expression -> expression.
+    Axiom instantiate : S.t -> Lifetime.t -> expression -> expression.
 
     Definition threadId := nat.
     Definition pool := list (threadId * expression * Lifetime.t).
@@ -57,11 +61,11 @@ Module Semantics (Lifetime : BoundedOrderedType).
 Inductive context : Type :=
     | CEmpty : context 
     | CSeq : context -> expression -> context 
-    | CBinding : variable -> context -> context 
+    | CBinding : Var.t -> context -> context 
     | CAssign : lval -> context -> context 
     | CBox : context -> context 
     | CTrc : context -> context 
-    | CSpawn : string -> list value -> context -> list expression -> context.
+    | CSpawn : Var.t -> list Value.value -> context -> list expression -> context.
 
 Fixpoint build (c : context) (e : expression) : expression :=
     match c with 
@@ -74,51 +78,60 @@ Fixpoint build (c : context) (e : expression) : expression :=
         | CSpawn f vl c el => ESpawn f ((List.map EVal vl)++[(build c e)]++el)
         end.
 
-    Definition lstate := Store.t * expression.
+    Definition lstate := S.t * expression.
 
+
+    Definition read (σ : S.t) (l : Lifetime.t) (ω : lval) : 
+        option (Value.partialValue * sum Lifetime.t nat) :=
+            S.loc σ l ω >>= S.get σ.
+    
+    Definition write (σ : S.t) (l : Lifetime.t) (ω : lval)  (v : Value.partialValue) : 
+        option S.t :=
+            S.loc σ l ω >>= (fun a => S.get σ a >>= (fun x =>  S.set σ a (v, snd x))).
+    
     Inductive step (p : program) (l : Lifetime.t) :
         transition lstate pool :=
             S_Copy : forall σ ω v m, 
-            Store.read σ l ω = Some (Some v, m) ->
+            read σ l ω = Some (Some v, m) ->
             step p l (σ, ERead Copy ω)  [] (σ, EVal v)
         |   S_Move : forall σ ω v σ' m, 
-            Store.read σ l ω = Some (Some v, m) ->
-            Store.write σ l ω None = Some σ' ->  
+            read σ l ω = Some (Some v, m) ->
+            write σ l ω None = Some σ' ->  
             step p l (σ, ERead Move ω) [] (σ', EVal v)
-        |   S_Box : forall  (σ σ' : Store.t) (m : nat) (v : value),
-            ~ Store.defined σ (inr m) ->
-            Store.allocate σ [(inr m, (Some v, inl Lifetime.glob))] = Some σ' -> 
-            step p l (σ, EBox v) [] (σ', EVal (Location (inr m) Owned))
-        |   S_Trc : forall  (σ σ' : Store.t) (m : nat) (v : value),
-            ~ Store.defined σ (inr m) ->
-            Store.allocate σ [(inr m, (Some v, inr 1))] = Some σ' -> 
+        |   S_Box : forall  (σ σ' : S.t) (m : nat) (v : value),
+            ~ S.defined σ (inr m) ->
+            S.allocate σ [(inr m, (Some v, inl Lifetime.glob))] = Some σ' -> 
+            step p l (σ, EBox v) [] (σ', EVal (Value.Location (inr m) Owned))
+        |   S_Trc : forall  (σ σ' : S.t) (m : nat) (v : value),
+            ~ S.defined σ (inr m) ->
+            S.allocate σ [(inr m, (Some v, inr 1))] = Some σ' -> 
             step p l (σ, ETrc v) [] (σ', EVal (Location (inr m) (Trc true)))
-        |   S_Clone : forall  (σ σ' : Store.t) (ω : lval) (m i : nat), 
-            Store.read σ l ω = Some (Some (Location (inr m) (Trc true)), inr i) ->
-            Store.clone σ l ω = Some σ' ->
+        |   S_Clone : forall  (σ σ' : S.t) (ω : lval) (m i : nat), 
+            read σ l ω = Some (Some (Location (inr m) (Trc true)), inr i) ->
+            S.clone σ l ω = Some σ' ->
             step p l (σ, EClone ω) [] (σ', EVal (Location (inr m) (Trc false)))
         |   S_Borrow : forall σ ω ℓ b,
-            Store.loc σ l ω = Some ℓ ->
+            S.loc σ l ω = Some ℓ ->
             step p l (σ, ERef b ω) [] (σ, EVal (Location ℓ Borrowed))
-        |   S_Declare : forall (σ σ' : Store.t) (x : variable) (v : value),
-            Store.write σ l (LVar x) (Some v) = Some σ' -> 
+        |   S_Declare : forall (σ σ' : S.t) (x : Var.t) (v : value),
+            write σ l (LVar x) (Some v) = Some σ' -> 
             step p l (σ, EBinding x v) [] (σ', EVal Unit)
-        |   S_Assign : forall (σ σ' σ'' : Store.t) (ω : lval) 
+        |   S_Assign : forall (σ σ' σ'' : S.t) (ω : lval) 
             (v:value) (v' : partialValue) m,
-            Store.read σ l ω = Some (v', m) -> 
-            Store.drop_val σ (Singleton _ v') = Some σ'' ->
-            Store.write σ'' l ω (Some v) = Some σ' ->
+            read σ l ω = Some (v', m) -> 
+            (* S.drop_val σ (Singleton _ v') = Some σ'' -> *)
+            write σ'' l ω (Some v) = Some σ' ->
             step p l (σ, EAssign ω (EVal v)) [] (σ', EVal Unit)
-        |   S_Seq : forall (σ σ' : Store.t) (v :value) (e1 e2  : expression),
-            Store.drop_val σ (Singleton _ (Some v)) = Some σ' ->
+        |   S_Seq : forall (σ σ' : S.t) (v :value) (e1 e2  : expression),
+            (* Store.drop_val σ (Singleton _ (Some v)) = Some σ' -> *)
             step p l (σ, ESeq (EVal v) e2) [] (σ, e2)
-        |   S_Block1 : forall ( m : Lifetime.t) (σ σ' : Store.t) (e e' : expression) T,
+        |   S_Block1 : forall ( m : Lifetime.t) (σ σ' : S.t) (e e' : expression) T,
             step p m (σ, e) T (σ', e') -> 
             step p l (σ, EBlock e m) T (σ', EBlock e' m)
-        |   S_Block2 : forall (m : Lifetime.t) (σ σ' : Store.t) (v : value),
-            Store.drop_lft σ m = Some σ' ->
+        |   S_Block2 : forall (m : Lifetime.t) (σ σ' : S.t) (v : value),
+            (* Store.drop_lft σ m = Some σ' -> *)
             step p l (σ, EBlock (EVal v) m) [] (σ, EVal v)
-        |   S_Spawn : forall (m m' : Lifetime.t) (σ σ' : Store.t) (f : String.string) (mth : method)
+        |   S_Spawn : forall (m m' : Lifetime.t) (σ σ' : S.t) (f : Var.t) (mth : method)
                 (e e' : expression) (el : list expression) (vl : list value) (t :threadId),
             functions p f = Some mth ->
             el = List.map EVal vl ->
@@ -126,15 +139,15 @@ Fixpoint build (c : context) (e : expression) : expression :=
             let xl := List.map (fun x =>  inl (fst x, m')) (params mth) in 
             let vl' := List.map (fun v => (Some v, inl m')) vl in
             let u := List.combine xl vl' in
-            Store.allocate σ u = Some σ' ->
+            S.allocate σ u = Some σ' ->
             step p l (σ, ESpawn f el) [(t, e', m')] (σ', EVal Unit).
 
     Definition run (p : program) (l : Lifetime.t) : 
         transition lstate (list (threadId * expression * Lifetime.t)) :=
-            tr_clos_rt _ _ (step p l).
+            reachable _ _ (step p l).
 
     
-    Inductive react (p : program) : relation (Store.t * pool) :=
+    Inductive react (p : program) : relation (S.t * pool) :=
         | react_done : forall σ, react p (σ, []) (σ, [])
         | react_step : forall l t σ σ' σ'' e e' T0 T T',
             step p l (σ, e) T0 (σ', e') -> 
@@ -156,13 +169,11 @@ Fixpoint build (c : context) (e : expression) : expression :=
                 | _, _ => False 
             end.
 
-    Definition instant (p : program) : relation (Store.t * pool) :=
+    Definition instant (p : program) : relation (S.t * pool) :=
         fun st st' =>
         let (σ, T) := st in 
         let (σ', T') := st' in
         exists T'', react p (σ, T) (σ', T') /\ resetAll T'' T'.
 
-    Definition reachable (p : program) : relation (Store.t * pool) :=
+    Definition reachable (p : program) : relation (S.t * pool) :=
         clos_refl_trans _ (instant p).
-
-End Semantics.
