theories/Store.v
@@ -1,0 +1,62 @@
+Require Import Lifetime.
+Require Import Ensembles.
+Require Import LVal.
+Module Type StoreDomain.
+    Parameter loc : Type.
+    Parameter val : Type.
+End StoreDomain.
+
+(* distinction set / write *)
+
+Module Store (Import D : StoreDomain).
+    (* address -> partialValue * sum lifetime nat *)
+    Parameter t : Type.
+    Parameter defined : t ->  loc -> Prop.
+    (* Parameter allocate : t -> location -> partialValue -> option t.*)
+    Parameter free : t -> loc -> option t.
+    
+    (* Parameter get : t -> location -> option partialValue.
+    Parameter set : t ->location -> partialValue -> option t.*)
+    
+    (*Parameter fetch : t -> variable -> Lifetime.t -> option (Lifetime.t).*)
+    (* Parameter get : t -> loc -> option (partialValue * sum Lifetime.t nat).  *)
+    Parameter get : t -> loc -> option val. 
+    Parameter set : t -> loc -> val -> option t.
+    Parameter allocate : t -> list (loc * val) -> option t.
+    
+    Parameter loc : t -> Lifetime.t -> lval -> option loc.
+    (* Parameter read : t -> Lifetime.t -> lval -> option val.
+    Parameter write : t -> Lifetime.t -> lval ->  value -> option t. *)
+    Parameter clone : t -> Lifetime.t -> lval -> option t.
+    
+    Parameter drop_val : t -> Ensemble val -> option t.
+    Parameter drop_lft : t -> Lifetime.t -> option t.
+    Parameter count : t -> nat -> option nat.
+    (* Parameter fetchprop : forall (x : variable) o m S,
+        fetch S x o = Some m ->
+        Lifetime.lt m o /\
+        forall n, defined S (inl (x, n)) -> not (Lifetime.lt n m).*)
+    (*   Parameter drop_prop1 : forall phi sigma,
+    Same_set value phi (Empty_set value) ->
+    drop sigma phi =  Some sigma.*)
+    
+    (*        Parameter drop_prop2 : forall phi v sigma l v' phi',
+    In _ phi (Location l Owned) ->
+    get sigma l = Some v' -> 
+    drop sigma phi = drop (free sigma l) (Union _ phi' (Singleton _ v')).
+    
+    Parameter drop_prop2 : forall phi phi' v sigma,
+    In _ phi v -> 
+    phi' = Subtract _ phi v ->
+    drop sigma phi = 
+    match v with 
+        | Location l Owned =>  
+            get sigma l = Some v'
+             (free sigma l)
+        | Location l Borrowed => Some sigma 
+        | Location l (Trc b) => Some (sigma)
+        | _ => drop sigma phi'
+    end.
+    (* we need the thread lifetime to fetch the variable *)
+    *)
+    End Store.
