theories/Types.v
@@ -1,0 +1,278 @@
+
+Require Import Coq.Relations.Relation_Definitions.
+Require Import Coq.Relations.Relation_Operators.
+Require Import Coq.Relations.Operators_Properties.
+Require Import Coq.Classes.RelationClasses.
+Require Import Coq.Program.Basics.
+Require Import Coq.Program.Equality.
+Require Import Coq.Sets.Ensembles.
+Require Import Coq.Lists.List.
+Require Import MSSL.Misc.
+Require Import MSSL.LVal MSSL.Lattice.
+
+Open Scope program_scope.
+
+    Inductive total : Type := 
+        | TUnit : total 
+        | TInt : total 
+        | TRef : bool -> Ensemble lval -> total
+        | TTRC : total -> total
+        | TBox : total -> total.
+
+    Inductive moved : Type :=
+        | TMoved : total -> moved
+        | TMBox : moved -> moved.
+    
+    Definition partial : Type := sum total moved.
+
+    Definition lift_total : total -> partial := (@inl total moved).
+    Definition lift_moved : moved -> partial := (@inr total moved).
+
+    Coercion lift_total : total >-> partial.
+    Coercion lift_moved : moved >-> partial.
+
+    Inductive lt : relation partial := 
+        | lt_unit : lt TUnit TUnit
+        | lt_int : lt TInt TInt
+        | lt_ref : forall b l1 l2,
+            Included _ l1 l2  -> lt (TRef b l1) (TRef b l2)
+        | lt_trc : forall (t1 t2 : total),
+            lt t1 t2 -> lt (TTRC t1) (TTRC t2)
+        | lt_box1 : forall (t1 t2 : total),
+            lt t1 t2 -> lt (TBox t1) (TBox t2) 
+        | lt_box2 : forall (t1 : total) (t2 : moved),
+            lt t1 t2 -> lt (TBox t1) (TMBox t2) 
+        | lt_box3 : forall (t1 t2 : moved),
+            lt t1 t2 -> lt (TMBox t1) (TMBox t2) 
+        | lt_undef1 : forall (t1 t2 : total),
+            lt t1 t2 -> lt (TMoved t1) (TMoved t2)
+        | lt_undef2 : forall (t1 t2 : total),
+            lt t1 t2 -> lt t1 (TMoved t2)
+        | lt_undef3 : forall (t1 : total) (t2 : total),
+            lt t1 (TMoved t2) -> lt (TBox t1) (TMoved (TBox t2))
+        | lt_undef4 : forall (t1 : moved) (t2 : total),
+            lt t1 (TMoved t2) -> lt (TMBox t1) (TMoved (TBox t2)).
+
+Lemma lt_moved_total : forall (t1 : moved) (t2 : total), lt t1 t2 -> False.
+Proof.
+    intros t1 t2 Ha.
+    dependent induction Ha.
+Qed.
+
+Lemma lt_moved : forall (t1 t2 : total), lt (inl t1) (TMoved t2) -> lt t1 t2.
+Proof.
+    intros t1 t2 Ha.
+    dependent induction Ha; auto using lt_box1, JMeq_refl.
+Qed.
+
+Lemma lt_refl : forall t, lt t t.
+Proof.
+    assert (forall t : total, lt t t) as Ha by
+        (induction t; auto using lt, reflexivity).
+    destruct t; [apply Ha | induction m; auto using lt]. 
+Qed.
+
+Lemma lt_trans : forall t1 t2, lt t1 t2 -> forall t3, lt t2 t3 -> lt t1 t3.
+Proof.
+    intros t1 t2 Ha.
+    dependent induction Ha; intros t3 Hb.
+    -   assumption.
+    -   assumption.
+    -   destruct t3 as [ [  ] | [ t |  ] ]; try solve [inversion Hb].
+        +   inversion Hb; subst.
+            eauto using lt_ref, transitivity.
+        +   dependent destruction Hb.
+            destruct t; try solve [inversion Hb].
+            inversion Hb; subst.
+            apply lt_undef2.
+            eauto using lt_ref, transitivity.
+    -   destruct t3 as [ [  ] | [ t |  ] ]; try solve [inversion Hb].
+        +   inversion Hb; subst.
+            *   apply lt_trc.
+                apply IHHa.
+                assumption.
+        +   dependent destruction Hb.
+            destruct t; try solve [inversion Hb].
+            inversion Hb; subst.
+            apply lt_undef2.
+            apply lt_trc; apply IHHa; assumption.
+    -   destruct t3 as [ [  ] | [ t |  ] ]; try solve [inversion Hb].
+        +   inversion Hb; subst.
+            apply lt_box1; apply IHHa; assumption.
+        +   dependent destruction Hb.
+            destruct t; try solve [inversion Hb].
+            inversion Hb; subst.
+            apply lt_undef2.
+            apply lt_box1; apply IHHa; assumption. 
+            * apply lt_undef2.
+                apply lt_box1.
+                apply IHHa.
+                apply lt_moved.
+                assumption.
+        +   inversion Hb; subst.
+            apply lt_box2.
+            apply IHHa; assumption.
+    -   destruct t3 as [ [  ] | [ t |  ] ]; try solve [inversion Hb].
+        +   destruct t; try solve [inversion Hb].
+            inversion Hb; subst.
+            apply lt_undef3.
+            apply IHHa; assumption.
+        +   apply lt_box2.
+            inversion Hb; subst.
+            apply IHHa; assumption.
+    -   destruct t3 as [ [  ] | [ t |  ] ]; try solve [inversion Hb].
+        +   destruct t; try solve [inversion Hb].
+            inversion Hb; subst.
+            apply lt_undef4.
+            apply IHHa; assumption.
+        +   apply lt_box3.
+            inversion Hb; subst.
+            apply IHHa; assumption.
+    -   destruct t3; [elim (lt_moved_total _ _ Hb) | ].
+        inversion Hb; subst.
+        apply lt_undef1.
+        apply IHHa; assumption. 
+    -   destruct t3; [elim (lt_moved_total _ _ Hb) | ].
+        inversion Hb; subst.
+        apply lt_undef2.
+        apply IHHa; assumption.
+    -   destruct t3; [elim (lt_moved_total _ _ Hb) | ].
+        inversion Hb; subst.
+        destruct t3; (try inversion H1).
+        subst.
+        apply lt_undef2.
+        apply lt_box1.
+        apply lt_moved.
+        apply IHHa.
+        constructor.
+        assumption.
+    -   destruct t3 ; [elim (lt_moved_total _ _ Hb) | ].
+        inversion Hb; subst.
+        destruct t3; (try inversion H1;subst).
+        apply lt_undef4.
+        apply IHHa.
+        apply lt_undef1; assumption.
+Qed.
+
+Lemma lt_antisymmetric_total : forall (t1 t2 : total), lt t1 t2 -> lt t2 t1 -> t1 = t2.
+Proof.
+    induction t1; intros.
+    -   inversion H; reflexivity.
+    -   inversion H; reflexivity.
+    -   inversion H; inversion H0; subst; try auto.
+        injection H5; intro; subst.
+        replace e with l2.
+        reflexivity.
+        apply Extensionality_Ensembles; unfold Same_set; auto.
+    -   inversion H; inversion H0; subst; try auto.
+        injection H4; intros; subst.
+        f_equal; eauto.
+    -   inversion H; inversion H0; subst; try auto.
+        injection H4; intros; subst.
+        f_equal; eauto.
+Qed.
+
+Lemma lt_antisymmetric_moved : forall (t1 t2 : moved), lt t1 t2 -> lt t2 t1 -> t1 = t2.
+Proof.
+    intros t1 t2. revert t1.
+    dependent induction t2; intros.
+    -   inversion H; subst.
+        +   inversion H0; subst.
+            *   f_equal.
+                now apply lt_antisymmetric_total.
+        +   inversion H0; subst.
+    -   inversion H; subst.
+        +   inversion H0; subst.
+            *   f_equal; auto.   
+Qed.             
+
+
+Lemma lt_antisymmetric : forall (t1 t2 : partial), lt t1 t2 -> lt t2 t1 -> t1 = t2.
+Proof.
+    intros t1 t2 Ha Hb.
+    destruct t1, t2.
+    -   f_equal.
+        apply lt_antisymmetric_total.
+        assumption.
+        assumption.
+    -   apply lt_moved_total in Hb.
+        elim Hb.
+    -   apply lt_moved_total in Ha.
+        elim Ha.
+    -   f_equal.
+        apply lt_antisymmetric_moved.
+        assumption.
+        assumption.
+Qed.
+
+Definition lt' (t1 t2 : option partial) : Prop :=
+    match (t1, t2) with
+        |   (Some t1, Some t2) => lt t1 t2
+        |   (None, _ ) => True 
+        |   (Some _, None ) => False
+    end.
+
+#[export] Instance lt_Reflexive : Reflexive lt'.
+Proof.
+    intro x.
+    destruct x; unfold lt'; auto using lt_refl.
+Qed.
+
+#[export] Instance lt_Transitive : Transitive lt'.
+Proof.
+    intros x y z H1 H2.
+    destruct x, y, z; unfold lt' in *; eauto using lt_trans.
+    elim H1.
+Qed.
+
+#[export] Instance lt_AntiSymmetric : Antisymmetric _ (@eq (option partial)) lt'.
+Proof.
+    intros x y Ha Hb.
+    destruct x, y.
+    f_equal.
+    now apply lt_antisymmetric.
+    inversion Ha.
+    inversion Hb.
+    reflexivity.
+Qed.
+
+#[export] Instance typePreorder : PreOrder lt'.
+constructor.
+apply lt_Reflexive.
+apply lt_Transitive.
+Qed.
+
+#[export] Instance PartialOrderlt : PartialOrder eq lt'.
+constructor.
+-   intro.
+    unfold relation_conjunction.
+    unfold predicate_intersection.
+    unfold pointwise_extension.
+    split; subst.
+    reflexivity.
+    unfold flip.
+    reflexivity.
+-   unfold relation_conjunction.
+    unfold predicate_intersection.
+    unfold pointwise_extension.
+    unfold lt'.
+    intros [Ha Hb].
+    unfold flip in Hb.
+    destruct x, x0.
+    f_equal.
+    apply lt_antisymmetric.
+    assumption.
+    assumption.
+    elim Ha.
+    elim Hb.
+    reflexivity.
+Qed.
+
+Fixpoint type_join (t1 t2 : option partial) : option partial := 
+    match t1, t2 with 
+        | _,_ => None 
+    end.
+
+#[export] Instance typeJoinLattice : JoinLattice (@eq (option partial)) lt' type_join.
+Admitted.
+
