theories/Variables.v
@@ -1,0 +1,10 @@
+Require Import String DecidableType.
+
+Module Var : DecidableType.
+    Definition t := String.string.
+    Definition eq := @eq String.string.
+    Definition eq_refl := @eq_refl String.string.
+    Definition eq_sym := @eq_sym String.string.
+    Definition eq_trans := @eq_trans String.string.
+    Definition eq_dec := String.string_dec.
+End Var.
